add initial proof that qsort sorts (both ordering and permutation properties)
Complete, except for the fact that antisymmetry and transitivity
should only be required for elements in the array range, not
any value of the type.

Also needs tidying and refactoring.

src/Init/Data/Array/QSort.lean
@@ -5,7 +5,30 @@ Authors: Leonardo de Moura
 -/
 prelude
 import Init.Data.Array.Basic
+import Init.Data.Array.Lemmas
 import Init.Data.Nat.Mod
+
+@[simp] theorem size_ite (P: Prop) [Decidable P] (a b: Array α): (if P then a else b).size = (if P then a.size else b.size) := by
+  split
+  all_goals rfl
+
+namespace Nat
+theorem avg_lt_of_lt (h: a < b): (a + b) / 2 < b := by
+  apply (Nat.div_lt_iff_lt_mul Nat.zero_lt_two).mpr
+  rw [Nat.mul_two]
+  exact Nat.add_lt_add_right h b
+
+theorem le_avg_of_le (h: a ≤ b): a ≤ (a + b) / 2 := by
+  apply (Nat.le_div_iff_mul_le _).mpr
+  · rw [Nat.mul_two]
+    exact Nat.add_le_add_left h a
+  · exact Nat.zero_lt_two
+
+theorem avg_le_of_le (h: a ≤ b): (a + b) / 2 ≤ b:= by
+  apply Nat.div_le_of_le_mul
+  rw [Nat.two_mul]
+  exact Nat.add_le_add_right h b
+end Nat
 
 namespace Array
 
@@ -29,10 +52,8 @@ namespace Array
 
       let mid := (low + high) / 2
 
-      have hms: mid < s := by
-        apply Nat.div_lt_of_lt_mul
-        rw [Nat.two_mul]
-        exact Nat.add_lt_add hls hhs
+      have hmh: mid ≤ high := Nat.avg_le_of_le hlh
+      have hms: mid < s := Nat.lt_of_le_of_lt hmh hhs
 
       let as := if lt (as[mid]'(hs ▸ hms)) (as[low]'(hs ▸ hls)) then as.swap ⟨low, hs ▸ hls⟩ ⟨mid, hs ▸ hms⟩ else as
       have hs: as.size = s := by dsimp only [as]; split; all_goals simp_all only [Array.size_swap]
@@ -45,7 +66,7 @@ namespace Array
 
       let pivot := as[high]'(hs ▸ hhs)
 
-      -- invariant: lo ≤ x < i → lt as[i] pivot, i ≤ x < j -> ¬lt as[i] pivot
+      -- invariant: lo ≤ k < i → lt as[i] pivot, i ≤ k < j -> ¬lt as[i] pivot
       let rec @[specialize] loop (as : Array α) (i j : Nat) (hli: low ≤ i) (hij: i ≤ j) (hjh: j ≤ high) (hhs: high < as.size): {as': Array α // as'.size = as.size}:=
         let s := as.size
         have hs: as.size = s := rfl
@@ -74,7 +95,7 @@ namespace Array
             ⟨as, hs⟩
         else if hih: i >= high then
           -- this can only happen if low == high assuming lt is antisymmetric
-          -- that's because i == j == high implies that all x in [low, high) are less than the pivot as[high]
+          -- that's because i == j == high implies that all k in [low, high) are less than the pivot as[high]
           -- in particular, this means that if mid != high, as[mid] is less than as[high], which is impossible,
           -- because we swap them in that case, so that a[mid] >= a[high]
           -- hence, mid = high, which implies (low + high) / 2 = high, which implies that low = high or
@@ -106,10 +127,562 @@ namespace Array
 
   (sort as low high hlh hhs).1
 
+@[simp] theorem size_qsort.sort (as : Array α) (lt : α → α → Bool) (low := 0) (high := as.size - 1)
+    (hlh: low ≤ high := by omega) (hhs: low < high → high < as.size := by omega):
+    (qsort.sort lt as low high hlh hhs).1.size = as.size := by
+  exact (qsort.sort lt as low high hlh hhs).2
+
 @[simp] theorem size_qsort (as : Array α) (lt : α → α → Bool) (low := 0) (high := as.size - 1)
     (hlh: low ≤ high := by omega) (hhs: low < high → high < as.size := by omega):
     (qsort as lt low high hlh hhs).size = as.size := by
   unfold qsort
   exact (qsort.sort lt as low high hlh hhs).2
+
+inductive IPerm {α} (low high: Nat): Array α → Array α → Prop where
+| refl: IPerm low high as as
+| swap (as: Array α) (i: Nat) (his: i < as.size) (hli: low ≤ i) (hih: i ≤ high) (j: Nat) (hjs: j < as.size) (hlj: low ≤ j) (hjh: j ≤ high): IPerm low high as (as.swap ⟨i, his⟩ ⟨j, hjs⟩)
+| trans {as as' as'': Array α}: IPerm low high as as' → IPerm low high as' as'' → IPerm low high as as''
+
+namespace IPerm
+theorem ite (p: Prop) [Decidable p] (low high: Nat) (as0 ast asf: Array α)
+    (hpt: IPerm low high as0 ast) (hpf: IPerm low high as0 asf):
+    IPerm low high as0 (if p then ast else asf) := by
+  split
+  case isTrue => exact hpt
+  case isFalse => exact hpf
+
+theorem dite (p: Prop) [Decidable p] (low high: Nat) (as0: Array α) (ast: p → Array α) (asf: ¬p → Array α)
+    (hpt: (h: p) → IPerm low high as0 (ast h)) (hpf: (h: ¬p) → IPerm low high as0 (asf h)):
+    IPerm low high as0 (if h: p then ast h else asf h) := by
+  split
+  case isTrue h => exact hpt h
+  case isFalse h => exact hpf h
+
+theorem trans_swap {as0 as: Array α} (hp: IPerm low high as0 as) (i: Nat) (his: i < as.size) (hli: low ≤ i) (hih: i ≤ high) (j: Nat) (hjs: j < as.size) (hlj: low ≤ j) (hjh: j ≤ high):
+  IPerm low high as0 (as.swap ⟨i, his⟩ ⟨j, hjs⟩) := by
+  apply IPerm.trans hp
+  apply IPerm.swap as i his hli hih j hjs hlj hjh
+
+theorem expand {α} {low high: Nat}
+    {low' high': Nat} (hll: low' ≤ low) (hhh: high ≤ high') {as: Array α} {as': Array α}
+    (p: IPerm low high as as'): IPerm low' high' as as' := by
+  induction p with
+  | refl => exact refl
+  | trans _ _ ih ih' => exact trans ih ih'
+  | swap as i his hli hih j hjs hlj hjh =>
+    exact swap as
+      i his (Nat.le_trans hll hli) (Nat.le_trans hih hhh)
+      j hjs (Nat.le_trans hll hlj) (Nat.le_trans hjh hhh)
+
+theorem size_eq {α} {as: Array α} {as': Array α} {low high: Nat}
+  (p: IPerm low high as as' ): as.size = as'.size := by
+  induction p with
+  | refl => rfl
+  | trans _ _ ih ih' => rwa [ih'] at ih
+  | swap => simp only [size_swap]
+
+def getElem?_lower {α: Type u} {as: Array α} {as': Array α} {low high: Nat} (hkl: k < low)
+  (p: IPerm low high as as'): as[k]? = as'[k]? := by
+  induction p with
+  | refl => rfl
+  | trans _ _ ih ih' => rwa [ih'] at ih
+  | swap _ _ _ hli _ _ _ hlj _ =>
+    simp [swap_def]
+    rw [getElem?_set_ne]
+    rw [getElem?_set_ne]
+    · exact Ne.symm (Nat.ne_of_lt (Nat.lt_of_lt_of_le hkl hli))
+    · exact Ne.symm (Nat.ne_of_lt (Nat.lt_of_lt_of_le hkl hlj))
+
+def getElem?_higher {α: Type u} {as: Array α} {as': Array α} {low high: Nat} (hhk: high < k)
+  (p: IPerm low high as as'): as[k]? = as'[k]? := by
+  induction p with
+  | refl => rfl
+  | trans _ _ ih ih' => rwa [ih'] at ih
+  | swap _ _ _ _ hih _ _ _ hjh =>
+    simp [swap_def]
+    rw [getElem?_set_ne]
+    rw [getElem?_set_ne]
+    · exact Nat.ne_of_lt (Nat.lt_of_le_of_lt hih hhk)
+    · exact Nat.ne_of_lt (Nat.lt_of_le_of_lt hjh hhk)
+end IPerm
+
+def IForAll (as: Array α) (P: α → Prop) (low high: Nat) :=
+  ∀ k, (hks: k < as.size) → low ≤ k → (hkh: k < high) → P (as[k]'hks)
+
+abbrev IForAllSwap (as: Array α) (i j) (his: i < as.size) (hjs: j < as.size) (P: α → Prop) (low high: Nat) :=
+  IForAll (as.swap ⟨i, his⟩ ⟨j, hjs⟩) P low high
+
+namespace IForAll
+theorem map {P: α → Prop} {Q: α → Prop} (ha: IForAll as P low high) (f: (a: α) → P a → Q a):
+  IForAll as Q low high := by
+  intro k hks hlk hkh
+  specialize ha k hks hlk hkh
+  exact f as[k] ha
+
+theorem swap_left {as: Array α} {P: α → Prop} {low: Nat} {i j: Nat}
+    (hij: i ≤ j) {hjs: j < as.size} (hjp: P (as[j]'hjs))
+    (ha: IForAll as P low i):
+    IForAllSwap as i j (Nat.lt_of_le_of_lt hij hjs) hjs P low (i + 1) := by
+  intro k hks hlk hki1
+  rw [size_swap] at hks
+  simp only [swap_def]
+  by_cases hki: k < i
+  · rw [getElem_set_ne]
+    rw [getElem_set_ne]
+    exact ha k hks hlk hki
+    · exact Ne.symm (Nat.ne_of_lt hki)
+    · have hkj: k < j := Nat.lt_of_lt_of_le hki hij
+      exact Ne.symm (Nat.ne_of_lt hkj)
+  · have hki: k = i := Nat.eq_of_lt_succ_of_not_lt hki1 hki
+    subst k
+    by_cases hij: i = j
+    · subst i
+      simp only [get_eq_getElem, getElem_set_eq]
+      exact hjp
+    rw [getElem_set_ne]
+    rw [getElem_set_eq]
+    simp only [get_eq_getElem]
+    exact hjp
+    · rfl
+    · intro h
+      exact hij (Eq.symm h)
+
+theorem swap_right {as: Array α} {P: α → Prop} {i j: Nat} (hij: i ≤ j) (hjs: j < as.size)
+    (hb: IForAll as P i j):
+    IForAllSwap as i j (Nat.lt_of_le_of_lt hij hjs) hjs P (i + 1) (j + 1) := by
+  intro k hks hi1x hkj1
+  rw [size_swap] at hks
+  simp only [swap_def]
+  by_cases hkj: k < j
+  · rw [getElem_set_ne]
+    rw [getElem_set_ne]
+    have hik: i ≤ k := Nat.le_of_succ_le hi1x
+    exact hb k hks hik hkj
+    · exact Nat.ne_of_lt hi1x
+    · exact Ne.symm (Nat.ne_of_lt hkj)
+  · have hkj: k = j := Nat.eq_of_lt_succ_of_not_lt hkj1 hkj
+    subst k
+    simp only [get_eq_getElem, getElem_set_eq]
+    exact hb i (Nat.lt_trans hi1x hjs) (Nat.le_refl i) hi1x
+
+theorem of_swap {as: Array α} {P: α → Prop} {low high i j: Nat} (hli: low ≤ i) (hij: i ≤ j) (hjh: j < high) {hjs: j < as.size}
+    (h: IForAllSwap as i j (Nat.lt_of_le_of_lt hij hjs) hjs
+      P low high): IForAll as P low high := by
+  have his := Nat.lt_of_le_of_lt hij hjs
+  intro k hks hlk hkh
+  simp [IForAllSwap, IForAll, size_swap, swap_def] at h
+  by_cases hki: k = i
+  · subst k
+    have hlj: low ≤ j := Nat.le_trans hli hij
+    specialize h j hjs hlj hjh
+    rwa [getElem_set_eq] at h
+    · rfl
+  by_cases hkj: k = j
+  · subst k
+    have hih: i < high := Nat.lt_of_le_of_lt hij hjh
+    specialize h i his hli hih
+    rw [getElem_set_ne] at h
+    rwa [getElem_set_eq] at h
+    · rfl
+    · exact hki
+  specialize h k hks hlk hkh
+  rw [getElem_set_ne] at h
+  rwa [getElem_set_ne] at h
+  · exact Ne.symm hki
+  · exact Ne.symm hkj
+
+/-- can use IPerm.expand if the sizes don't match --/
+theorem transport_in {low high : Nat} {as as' : Array α}
+    (hp : IPerm low high as as')
+    (h : as.IForAll P low (high + 1)):
+    as'.IForAll P low (high + 1) := by
+  induction hp with
+  | refl => exact h
+  | trans _ _ ih ih' => exact ih' (ih h)
+  | swap as i his hli hih j hjs hlj hjh  =>
+    intro k hks hlk hkh
+    simp [swap_def]
+    rw [getElem_set]
+    rw [getElem_set]
+    split
+    · exact h i his hli (Nat.lt_add_one_of_le hih)
+    · split
+      · exact h j hjs hlj (Nat.lt_add_one_of_le hjh)
+      · simp [size_swap] at hks
+        exact h k hks hlk hkh
+
+/-- can use IPerm.expand if the endpoints don't match --/
+theorem transport_lower {low high : Nat} {as as' : Array α}
+    (hp : IPerm low high as as')
+    (h : as.IForAll P begin low):
+    as'.IForAll P begin low := by
+induction hp with
+| refl => exact h
+| trans _ _ ih ih' => exact ih' (ih h)
+| swap as i his hli _ j hjs hlj _  =>
+  intro k hks hbk hkl
+  simp [swap_def]
+  rw [getElem_set_ne]
+  rw [getElem_set_ne]
+  · simp [size_swap] at hks
+    exact h k hks hbk hkl
+  · exact Ne.symm (Nat.ne_of_lt (Nat.lt_of_lt_of_le hkl hli))
+  · exact Ne.symm (Nat.ne_of_lt (Nat.lt_of_lt_of_le hkl hlj))
+
+/-- can use IPerm.expand if the endpoints don't match --/
+theorem transport_higher {low high : Nat} {as as' : Array α}
+    (hp : IPerm low high as as')
+    (h : as.IForAll P (high + 1) ends):
+    as'.IForAll P (high + 1) ends := by
+induction hp with
+| refl => exact h
+| trans _ _ ih ih' => exact ih' (ih h)
+| swap as i his _ hih j hjs _ hjh  =>
+  intro k hks hhk hke
+  simp [swap_def]
+  rw [getElem_set_ne]
+  rw [getElem_set_ne]
+  · simp [size_swap] at hks
+    exact h k hks hhk hke
+  · exact Nat.ne_of_lt (Nat.lt_of_le_of_lt hih hhk)
+  · exact Nat.ne_of_lt (Nat.lt_of_le_of_lt hjh hhk)
+
+end IForAll
+
+def IsAsymm {α} (r: α → α → Prop) :=
+  {x: α} → {y: α} → r x y → r y x → False
+
+def IsTrans {α} (r: α → α → Prop) :=
+  {x: α} → {y: α} → {z: α} → r x y → r y z → r x z
+
+def IOrdered (lt: α → α → Bool) (low: Nat) (high: Nat) (as: Array α) :=
+  ∀ i j, (hli: low ≤ i) → (hij: i < j) → (hjh: j ≤ high) → (hjs: j < as.size) →
+  lt (as[j]'hjs) (as[i]'(Nat.lt_trans hij hjs)) = false
+
+namespace IOrdered
+theorem mkSingle (lt : α → α → Bool) (k: Nat) (as: Array α):
+    IOrdered lt k k as := by
+  unfold IOrdered
+  intro i j hli hij hjl hjs
+  exfalso
+  have hkk: k < k := Nat.lt_of_le_of_lt hli (Nat.lt_of_lt_of_le hij hjl)
+  exact (Nat.ne_of_lt hkk) rfl
+
+theorem restrict {low high: Nat}
+    {low' high': Nat} (hll: low ≤ low') (hhh: high' ≤ high) {as: Array α}
+    (p: IOrdered lt low high as): IOrdered lt low' high' as := by
+  unfold IOrdered
+  intro i j hli hij hjl hjs
+  exact p i j (Nat.le_trans hll hli) hij (Nat.le_trans hjl hhh) hjs
+
+/-- can use IPerm.expand if the endpoints don't match --/
+theorem transport_lower {low high : Nat} {as as' : Array α}
+    (hp : IPerm (low + 1) high as as')
+    (h : as.IOrdered lt begin low):
+    as'.IOrdered lt begin low := by
+induction hp with
+| refl => exact h
+| trans _ _ ih ih' => exact ih' (ih h)
+| swap as i his hli _ j hjs hlj _ =>
+  intro a b hla hab hbl hbs
+  have hal := Nat.lt_of_lt_of_le hab hbl
+  simp [swap_def]
+  rw [getElem_set_ne]
+  rw [getElem_set_ne]
+  rw [getElem_set_ne]
+  rw [getElem_set_ne]
+  · simp [size_swap] at hbs
+    exact h a b hla hab hbl hbs
+  · exact Ne.symm (Nat.ne_of_lt (Nat.lt_trans hal hli))
+  · exact Ne.symm (Nat.ne_of_lt (Nat.lt_trans hal hlj))
+  · exact Ne.symm (Nat.ne_of_lt (Nat.lt_of_le_of_lt hbl hli))
+  · exact Ne.symm (Nat.ne_of_lt (Nat.lt_of_le_of_lt hbl hlj))
+
+theorem glue
+    {lt : α → α → Bool} {low high : Nat} {pivot : α} {i : Nat} {as : Array α}
+    (ha : as.IForAll (fun x => lt pivot x = false) low (i + 1))
+    (hb : as.IForAll (fun x => lt x pivot = false) (i + 1) (high + 1))
+    (hlttr : IsTrans fun x x_1 => lt x x_1 = false)
+    (h1 : IOrdered lt low i as)
+    (h2 : IOrdered lt (i + 1) high as):
+    IOrdered lt low high as := by
+  unfold IOrdered
+  intro a b hla hab hbh hbs
+  have has := Nat.lt_trans hab hbs
+
+  by_cases hbi: b ≤ i
+  · exact h1 a b hla hab hbi hbs
+
+  have hib: i < b := Nat.succ_le_of_lt (Nat.gt_of_not_le hbi)
+  by_cases hia: i + 1 ≤ a
+  · exact h2 a b hia hab hbh hbs
+
+  have hai: a < i + 1 := by exact Nat.gt_of_not_le hia
+  specialize ha a has hla hai
+  specialize hb b hbs hib (Nat.lt_add_one_of_le hbh)
+  exact hlttr hb ha
+
+end IOrdered
+
+abbrev swap_getElem (as: Array α) (i j k: Nat) (his: i < as.size) (hjs: j < as.size) (hks: k < as.size): α :=
+  (as.swap ⟨i, his⟩ ⟨j, hjs⟩)[k]'(
+      le_of_le_of_eq hks (Eq.symm (size_swap as ⟨i, his⟩ ⟨j, hjs⟩))
+    )
+
+theorem getElem_after_swap {as: Array α} {i j high: Nat} (hij: i ≤ j) (hjh: j < high) (hhs: high < as.size):
+    as.swap_getElem i j high (Nat.lt_of_le_of_lt hij (Nat.lt_trans hjh hhs)) (Nat.lt_trans hjh hhs) hhs
+    = (as[high]'hhs) := by
+  simp [swap_getElem, swap_def]
+  rw [getElem_set_ne]
+  rw [getElem_set_ne]
+  · exact Nat.ne_of_lt (Nat.lt_of_le_of_lt hij hjh)
+  · exact Nat.ne_of_lt (hjh)
+
+structure ISortOf (lt: α → α → Bool) (low high: Nat) (orig: Array α) (sorted: Array α): Prop where
+  perm: IPerm low high orig sorted
+  ord: IOrdered lt low high sorted
+
+namespace ISortOf
+theorem mkSingle (lt : α → α → Bool) (k: Nat) (as0: Array α) (as: Array α) (hp: IPerm k k as0 as):
+    ISortOf lt k k as0 as := ⟨hp, IOrdered.mkSingle lt k as⟩
+
+theorem trans {lt: α → α → Bool} {low high: Nat} {as as' as'': Array α}
+    (hp: IPerm low high as as') (hs: ISortOf lt low high as' as''):
+    (ISortOf lt low high as as'') := by
+    constructor
+    case ord =>
+      exact hs.ord
+    case perm =>
+      apply IPerm.trans hp hs.perm
+end ISortOf
+
+mutual
+  theorem qsort_sort_sort_sorts (lt : α → α → Bool) (low high : Nat) (pivot : α) (i : Nat) (as0: Array α) (as: Array α) (hp: IPerm low high as0 as)
+      (hli : low ≤ i) (hih : i < high) (hhs : high < as.size)
+      (ha: IForAll as (lt pivot · = false) low (i + 1))
+      (hb: IForAll as (lt · pivot = false) (i + 1) (high + 1))
+      (hltas: IsAsymm (lt · ·)) (hlttr: IsTrans (lt · · = false)):
+      have ⟨as', hs'⟩ := qsort.sort lt as low i hli (λ _ ↦ Nat.lt_trans hih hhs)
+      ISortOf lt low high as0 (qsort.sort lt as' (i + 1) high hih (λ _ ↦ hs' ▸ hhs)) := by
+
+    have h1 := qsort_sort_sorts as lt low i hli (λ _ ↦ Nat.lt_trans hih hhs) hltas hlttr
+    let ahs' := qsort.sort lt as low i hli (λ _ ↦ Nat.lt_trans hih hhs)
+    let as' := ahs'.1
+    let hs' := ahs'.2
+    have h2 := qsort_sort_sorts as' lt (i + 1) high hih (λ _ ↦ hs' ▸ hhs) hltas hlttr
+    constructor
+    case perm =>
+      apply IPerm.trans hp
+      apply IPerm.trans
+      · apply IPerm.expand (Nat.le_refl _) (Nat.le_of_lt hih) h1.perm
+      · apply IPerm.expand (Nat.le_add_right_of_le hli) (Nat.le_refl _) h2.perm
+
+    case ord =>
+      apply IOrdered.glue
+      case hlttr => exact hlttr
+      case pivot => exact pivot
+      case i => exact i
+      case ha => exact (ha.transport_in h1.perm).transport_lower h2.perm
+      case hb => exact (hb.transport_higher h1.perm).transport_in h2.perm
+      case h1 =>
+        apply IOrdered.transport_lower
+        case hp => exact h2.perm
+        case h => exact h1.ord
+      case h2 => exact h2.ord
+      termination_by (high - low, 0, 0)
+
+  theorem qsort_sort_loop_sorts (lt : α → α → Bool) (low high : Nat) (as0: Array α) (as: Array α) (hp: IPerm low high as0 as)
+      {pivot : α} (i j : Nat)
+      (hli : low ≤ i) (hij : i ≤ j) (hjh : j ≤ high) (hhs : high < as.size) (hph: as[high]'hhs = pivot)
+      (ha: IForAll as (lt · pivot) low i)
+      (hb: IForAll as (lt · pivot = false) i j)
+      (hc: IForAll as (lt · pivot) low high → low = high)
+      (hltas: IsAsymm (lt · ·)) (hlttr: IsTrans (lt · · = false)):
+      ISortOf lt low high as0 (qsort.sort.loop lt low high pivot as i j hli hij hjh hhs) := by
+    unfold qsort.sort.loop
+
+    have hjs: j < as.size := Nat.lt_of_le_of_lt hjh hhs
+    have his: i < as.size := Nat.lt_of_le_of_lt hij hjs
+    have hih: i ≤ high := Nat.le_trans hij hjh
+    have hlj: low ≤ j := Nat.le_trans hli hij
+    have hlh: low ≤ high := Nat.le_trans hli hih
+
+    by_cases hjh': j < high
+    all_goals simp only [hjh', ↓reduceDIte]
+
+    case pos =>
+      have hjs: j < as.size := Nat.lt_trans hjh' hhs
+      by_cases hjp: lt (as[j]'hjs) pivot = true
+      all_goals simp only [hjp, Bool.false_eq_true, ↓reduceIte]
+
+      case pos =>
+        apply qsort_sort_loop_sorts
+        case hph => simpa only [getElem_after_swap hij hjh' hhs]
+        case ha => exact ha.swap_left hij hjp
+        case hb => exact hb.swap_right hij hjs
+        case hc => intro h; apply hc; exact h.of_swap hli hij hjh'
+        case hltas => exact hltas
+        case hlttr => exact hlttr
+        case hp => exact .trans hp (.swap as i his hli hih j hjs hlj hjh)
+
+      case neg =>
+        apply qsort_sort_loop_sorts
+        case hph => exact hph
+        case ha =>
+          exact ha
+
+        case hb =>
+          intro k hks hik hkj1
+          by_cases hkj: k < j
+          · specialize hb k hks hik hkj
+            exact hb
+          · have hkj: k = j := Nat.eq_of_lt_succ_of_not_lt hkj1 hkj
+            subst k
+            exact eq_false_of_ne_true hjp
+
+        case hc =>
+          exact hc
+
+        case hltas => exact hltas
+        case hlttr => exact hlttr
+        case hp => exact hp
+
+    case neg =>
+      have hjh: j = high := Nat.le_antisymm hjh (Nat.le_of_not_lt hjh')
+      subst j
+      by_cases hhi: i ≥ high
+      all_goals simp only [hhi, ↓reduceDIte]
+
+      case pos =>
+        have hih: i ≤ high := Nat.le_trans hij hjh
+        have hi: i = high := Nat.le_antisymm hih hhi
+        subst i
+        suffices h: low = high by
+          subst high
+          apply ISortOf.mkSingle
+          exact hp
+
+        apply hc
+        exact ha
+
+      case neg =>
+        apply qsort_sort_sort_sorts
+        case hhs => simpa [size_swap]
+        case hp =>
+          exact IPerm.trans_swap hp i his hli hih high hhs hlh (Nat.le_refl _)
+        case ha =>
+          let ha := ha.map (λ x a ↦ eq_false_of_ne_true (hltas a))
+
+          have hhh: lt as[high] as[high] = false := by
+            exact eq_false_of_ne_true fun a => hltas a a
+
+          exact (hph ▸ ha).swap_left hij hhh
+        case hb => exact (hph ▸ hb).swap_right hij hhs
+        case hltas => exact hltas
+        case hlttr => exact hlttr
+        termination_by (high - low, 1, high - j)
+
+  theorem qsort_sort_loop_pivot_swap_sorts (lt : α → α → Bool) (low high : Nat) (as0: Array α) (as: Array α) (hp: IPerm low high as0 as)
+      (mid: Nat) (hlm: low ≤ mid) (hmh: mid < high) (hhs : high < as.size)
+      --(hltas: lt as[mid] as[high] = true → lt as[high] as[mid] = true → False)
+      (hltas: IsAsymm (lt · ·)) (hlttr: IsTrans (lt · · = false)):
+
+      let as' := if lt (as[mid]'(Nat.lt_trans hmh hhs)) (as[high]'hhs) then as.swap ⟨mid, Nat.lt_trans hmh hhs⟩ ⟨high, hhs⟩ else as
+      have hs': as'.size = as.size := by dsimp only [as']; split; all_goals simp_all only [Array.size_swap]
+
+      ISortOf lt low high as0 (qsort.sort.loop lt low high (as'[high]'(hs' ▸ hhs)) as' low low
+        (Nat.le_refl low) (Nat.le_refl low) (Nat.le_trans hlm (Nat.le_of_lt hmh)) (hs' ▸ hhs)).1 := by
+    have hms := Nat.lt_trans hmh hhs
+    have hlh := Nat.le_trans hlm (Nat.le_of_lt hmh)
+
+    have hmh': mid ≠ high := Nat.ne_of_lt hmh
+    apply qsort_sort_loop_sorts
+    case hc =>
+      intro h
+      simp only [IForAll, size_ite, size_swap, ite_self] at h
+      specialize h mid hms hlm hmh
+      simp [swap_def] at h
+      split at h
+      case isTrue h' =>
+        rw [getElem_set_ne] at h
+        rw [getElem_set_eq] at h
+        rw [getElem_set_eq] at h
+        exfalso
+        exact hltas h' h
+        · rfl
+        · rfl
+        · exact Ne.symm hmh'
+      case isFalse h' =>
+        exfalso
+        exact h' h
+    case hph => rfl
+    case hltas => exact hltas
+    case hlttr => exact hlttr
+    case hp =>
+      split
+      case isTrue h =>
+        exact .trans hp <| .swap as mid hms hlm (Nat.le_of_lt hmh) high hhs hlh (Nat.le_refl _)
+      case isFalse h =>
+        exact hp
+    all_goals
+      intro k hks hlk hkl
+      have hll: low < low := Nat.lt_of_le_of_lt hlk hkl
+      exfalso
+      exact (Nat.ne_of_lt hll) rfl
+      termination_by (high - low, 2, 0)
+
+  theorem qsort_sort_sorts (as: Array α) (lt : α → α → Bool) (low := 0) (high := as.size - 1)
+      (hlh: low ≤ high := by omega) (hhs: low < high → high < as.size := by omega)
+      -- TODO: to use this less constrained version, we need proofs that as'es are a permutation of eac hother
+      --(hltas: {i: Nat} → (hli: low ≤ i) → (hih: i ≤ high) → {j: Nat} → (hlj: low ≤ j) → (hjh: j ≤ high) → lt as[i] as[j] = true → lt as[j] as[i] = true → False):
+      (hltas: IsAsymm (lt · ·)) (hlttr: IsTrans (lt · · = false)):
+      ISortOf lt low high as (qsort.sort lt as low high hlh hhs) := by
+      unfold qsort.sort
+      by_cases hlh': low ≥ high
+      case pos =>
+        simp [hlh']
+        constructor
+        case ord =>
+          intro i j hli hij hjh hjs
+          have hlh := Nat.lt_of_le_of_lt hli (Nat.lt_of_lt_of_le hij hjh)
+          exfalso
+          have hlh'': ¬(low ≥ high) := by
+            exact Nat.not_le_of_lt hlh
+          exact hlh'' hlh'
+        case perm =>
+          exact IPerm.refl
+      case neg =>
+        simp only [hlh']
+        have hlh': low < high := Nat.gt_of_not_le hlh'
+
+        apply qsort_sort_loop_pivot_swap_sorts
+
+        case hlm => exact Nat.le_avg_of_le hlh
+        case hmh => exact Nat.avg_lt_of_lt hlh'
+
+        case hltas => exact hltas
+        case hlttr => exact hlttr
+
+        case hp =>
+          repeat any_goals
+            first
+            | apply Nat.le_refl
+            | apply Nat.avg_le_of_le
+            | apply Nat.le_avg_of_le
+            | apply IPerm.refl
+            | apply IPerm.ite
+            | apply IPerm.trans_swap
+            | assumption
+    termination_by ((sizeOf high) - (sizeOf low), 3, 0)
+end
+
+theorem qsort_sorts (as: Array α) (lt : α → α → Bool) (low := 0) (high := as.size - 1)
+    (hlh: low ≤ high := by omega) (hhs: low < high → high < as.size := by omega)
+    (hltas: IsAsymm (lt · ·)) (hlttr: IsTrans (lt · · = false)):
+    ISortOf lt low high as (qsort as lt low high hlh hhs)  := by
+    unfold qsort
+    apply qsort_sort_sorts
+    · exact hltas
+    · exact hlttr
 
 end Array
